changed OTypeExpr to be indexed by the type and OTRelation it represents; do not quite have osimpl working again...

theories/TypeReflection/OExpr.v
@@ -1,6 +1,8 @@
 Require Export PredMonad.TypeReflection.OrderedType.
 Require Export PredMonad.TypeReflection.OTypeExpr.
 
+Import EqNotations.
+
 
 (***
  *** Helper Tactics
@@ -17,26 +19,30 @@ Ltac split_ands :=
  *** Ordered Expressions
  ***)
 
-Inductive OVar A : Ctx -> Type :=
-| OVar_0 {ctx:Ctx} : OVar A (CtxCons A ctx)
-| OVar_S {ctx:Ctx} {B} : OVar A ctx -> OVar A (CtxCons B ctx)
+Inductive OVar {A RA} (tpA:@OTypeExpr A RA) : Ctx -> Type :=
+| OVar_0 {ctx} : OVar tpA (@CtxCons A RA tpA ctx)
+| OVar_S {B RB tpB ctx} : OVar tpA ctx -> OVar tpA (@CtxCons B RB tpB ctx)
 .
 
-Arguments OVar_0 {A ctx}.
-Arguments OVar_S {A ctx B} v.
+Arguments OVar_0 {A RA tpA ctx}.
+Arguments OVar_S {A RA tpA B RB tpB ctx} v.
 
 (* Expressions to represent proper functions *)
-Inductive OExpr (ctx:Ctx) : OTypeExpr -> Type :=
-| Var {A} (v:OVar A ctx) : OExpr ctx A
-| Embed {A:OTypeExpr} (a:A) : OExpr ctx A
-| App {A B} (e1 : OExpr ctx (OTpArrow A B)) (e2 : OExpr ctx A) : OExpr ctx B
-| Lam {A B} (e: OExpr (CtxCons A ctx) B) : OExpr ctx (OTpArrow A B)
+Inductive OExpr ctx : forall {A RA}, @OTypeExpr A RA -> Type :=
+| Var {A RA tp} (v:OVar tp ctx) : @OExpr ctx A RA tp
+| Embed {A RA tp} (a:A) : @OExpr ctx A RA tp
+| App {A RA} {tpA:@OTypeExpr A RA} {B RB} {tpB:@OTypeExpr B RB}
+      (e1 : OExpr ctx (OTpArrow tpA tpB)) (e2 : OExpr ctx tpA) :
+    OExpr ctx tpB
+| Lam {A RA} {tpA:@OTypeExpr A RA} {B RB} {tpB:@OTypeExpr B RB}
+      (e: OExpr (CtxCons tpA ctx) tpB) :
+    OExpr ctx (OTpArrow tpA tpB)
 .
 
-Arguments Var {ctx A} v.
-Arguments Embed {ctx A} a.
-Arguments App {ctx A B} e1 e2.
-Arguments Lam {ctx A B} e.
+Arguments Var {ctx A RA tp} v.
+Arguments Embed {ctx A RA tp} a.
+Arguments App {ctx A RA tpA B RB tpB} e1 e2.
+Arguments Lam {ctx A RA tpA B RB tpB} e.
 
 
 (***
@@ -44,23 +50,23 @@ Arguments Lam {ctx A B} e.
  ***)
 
 (* The semantics of a variable *)
-Fixpoint varSemantics {A ctx} (v:OVar A ctx) :
+Fixpoint varSemantics {A RA tp ctx} (v:@OVar A RA tp ctx) :
   CtxElem ctx -o> A :=
   match v in OVar _ ctx return CtxElem ctx -o> A with
   | OVar_0 => ctx_head_pfun
   | OVar_S v' => compose_pfun ctx_tail_pfun (varSemantics v')
   end.
-Arguments varSemantics {A ctx} !v.
+Arguments varSemantics {A RA tp ctx} !v.
 
 (* The semantics of an ordered expression *)
-Fixpoint exprSemantics {ctx A} (e:OExpr ctx A) : CtxElem ctx -o> A :=
-  match e in OExpr _ A return CtxElem ctx -o> A with
+Fixpoint exprSemantics {ctx A RA tp} (e:@OExpr ctx A RA tp) : CtxElem ctx -o> A :=
+  match e in @OExpr _ A RA tp return CtxElem ctx -o> A with
   | Var v => varSemantics v
   | Embed a => const_pfun a
   | App e1 e2 => pfun_apply (exprSemantics e1) (exprSemantics e2)
   | Lam e => pfun_curry (exprSemantics e)
   end.
-Arguments exprSemantics {ctx A} !e.
+Arguments exprSemantics {ctx A RA tp} !e.
 
 
 (***
@@ -68,12 +74,12 @@ Arguments exprSemantics {ctx A} !e.
  ***)
 
 (* Two expressions are related iff their semantics are *)
-Definition oexpr_R {ctx A} (e1 e2:OExpr ctx A) : Prop :=
+Definition oexpr_R {ctx A RA tp} (e1 e2:@OExpr ctx A RA tp) : Prop :=
   exprSemantics e1 <o= exprSemantics e2.
-Arguments oexpr_R {ctx A} e1 e2 : simpl never.
+Arguments oexpr_R {ctx A RA tp} e1 e2 : simpl never.
 
 (* oexpr_R is a PreOrder *)
-Instance PreOrder_oexpr_R ctx A : PreOrder (@oexpr_R ctx A).
+Instance PreOrder_oexpr_R ctx A RA tp : PreOrder (@oexpr_R ctx A RA tp).
 Proof.
   unfold oexpr_R; split; intro; intros.
   - reflexivity.
@@ -81,12 +87,12 @@ Proof.
 Qed.
 
 (* Two expressions are equivalenct iff their semantics are *)
-Definition oexpr_eq {ctx A} (e1 e2:OExpr ctx A) : Prop :=
+Definition oexpr_eq {ctx A RA tp} (e1 e2:@OExpr ctx A RA tp) : Prop :=
   exprSemantics e1 =o= exprSemantics e2.
-Arguments oexpr_eq {ctx A} e1 e2 : simpl never.
+Arguments oexpr_eq {ctx A RA tp} e1 e2 : simpl never.
 
 (* oexpr_eq is a Equivalence *)
-Instance Equivalence_oexpr_eq ctx A : Equivalence (@oexpr_eq ctx A).
+Instance Equivalence_oexpr_eq ctx A RA tp : Equivalence (@oexpr_eq ctx A RA tp).
 Proof.
   unfold oexpr_eq; split; intro; intros.
   - reflexivity.
@@ -101,47 +107,47 @@ Notation "x =e= y" :=
 
 
 (* The Embed constructor is Proper w.r.t. ot_R and oexpr_R *)
-Instance Proper_Embed ctx A :
-  Proper (ot_R ==> oexpr_R) (@Embed ctx A).
+Instance Proper_Embed ctx A RA tp :
+  Proper (ot_R ==> oexpr_R) (@Embed ctx A RA tp).
 Proof.
   intros a1 a2 Ra; unfold oexpr_R; simpl.
   apply Proper_const_pfun. assumption.
 Qed.
 
 (* The Embed constructor is Proper w.r.t. ot_equiv and oexpr_eq *)
-Instance Proper_Embed_equiv ctx A :
-  Proper (ot_equiv ==> oexpr_eq) (@Embed ctx A).
+Instance Proper_Embed_equiv ctx A RA tp :
+  Proper (ot_equiv ==> oexpr_eq) (@Embed ctx A RA tp).
 Proof.
   intros a1 a2 Ra. destruct Ra; split; apply Proper_Embed; assumption.
 Qed.
 
 (* The App constructor is Proper *)
-Instance Proper_App ctx A B :
-  Proper (oexpr_R ==> oexpr_R ==> oexpr_R) (@App ctx A B).
+Instance Proper_App ctx A RA tpA B RB tpB :
+  Proper (oexpr_R ==> oexpr_R ==> oexpr_R) (@App ctx A RA tpA B RB tpB).
 Proof.
   intros f1 f2 Rf a1 a2 Ra. unfold oexpr_R; simpl.
   apply Proper_pfun_apply; assumption.
 Qed.
 
 (* The App constructor is Proper for equivalence *)
-Instance Proper_App_equiv ctx A B :
-  Proper (oexpr_eq ==> oexpr_eq ==> oexpr_eq) (@App ctx A B).
+Instance Proper_App_equiv ctx A RA tpA B RB tpB :
+  Proper (oexpr_eq ==> oexpr_eq ==> oexpr_eq) (@App ctx A RA tpA B RB tpB).
 Proof.
   intros f1 f2 Rf a1 a2 Ra. unfold oexpr_eq; simpl.
   apply Proper_pfun_apply_equiv; assumption.
 Qed.
 
 (* The Lam constructor is Proper *)
-Instance Proper_Lam ctx {A B} :
-  Proper (oexpr_R ==> oexpr_R) (@Lam ctx A B).
+Instance Proper_Lam ctx A RA tpA B RB tpB :
+  Proper (oexpr_R ==> oexpr_R) (@Lam ctx A RA tpA B RB tpB).
 Proof.
   intros e1 e2 Re. unfold oexpr_R; simpl.
   apply Proper_pfun_curry. assumption.
 Qed.
 
 (* The Lam constructor is Proper for equivalence *)
-Instance Proper_Lam_equiv ctx {A B} :
-  Proper (oexpr_eq ==> oexpr_eq) (@Lam ctx A B).
+Instance Proper_Lam_equiv ctx A RA tpA B RB tpB :
+  Proper (oexpr_eq ==> oexpr_eq) (@Lam ctx A RA tpA B RB tpB).
 Proof.
   intros e1 e2 Re. unfold oexpr_eq; simpl.
   apply Proper_pfun_curry_equiv. assumption.
@@ -153,21 +159,23 @@ Qed.
  ***)
 
 (* Weakening / lifting of ordered expression variables *)
-Fixpoint weakenOVar w tpW :
-  forall {ctx A}, OVar A ctx -> OVar A (ctxInsert w tpW ctx) :=
-  match w return forall ctx A, OVar A ctx -> OVar A (ctxInsert w tpW ctx) with
-  | 0 => fun _ _ v => OVar_S v
+Fixpoint weakenOVar w {W RW} (tpW:@OTypeExpr W RW) :
+  forall {ctx A RA tpA}, @OVar A RA tpA ctx -> OVar tpA (ctxInsert w tpW ctx) :=
+  match w return forall ctx A RA tpA,
+      OVar tpA ctx -> OVar tpA (ctxInsert w tpW ctx) with
+  | 0 => fun _ _ _ _ v => OVar_S v
   | S w' =>
-    fun ctx A v =>
-      match v in OVar _ ctx return OVar A (ctxInsert (S w') tpW ctx) with
+    fun ctx A RA tpA v =>
+      match v in OVar _ ctx return OVar tpA (ctxInsert (S w') tpW ctx) with
       | OVar_0 => OVar_0
       | OVar_S v' => OVar_S (weakenOVar w' tpW v')
       end
   end.
+Arguments weakenOVar w {W RW} tpW {ctx A RA tpA} v : simpl nomatch.
 
 (* Correctness of weakenOVar: it is equivalent to weaken_pfun *)
-Lemma weakenOVar_correct w tpW {ctx A} (v:OVar A ctx) :
-  varSemantics (weakenOVar w tpW v) =o=
+Lemma weakenOVar_correct w {W RW} tpW {ctx A RA tpA} (v:@OVar A RA tpA ctx) :
+  varSemantics (@weakenOVar w W RW tpW ctx A RA tpA v) =o=
   compose_pfun (weaken_pfun w tpW ctx) (varSemantics v).
 Proof.
   revert ctx v; induction w; intros; [ | destruct v ]; simpl.
@@ -178,8 +186,8 @@ Proof.
 Qed.
 
 (* Weakening / lifting of ordered expressions *)
-Fixpoint weakenOExpr w tpW {ctx A} (e:OExpr ctx A)
-  : OExpr (ctxInsert w tpW ctx) A :=
+Fixpoint weakenOExpr w {W RW} (tpW:@OTypeExpr W RW) {ctx A RA tpA}
+         (e:@OExpr ctx A RA tpA) : OExpr (ctxInsert w tpW ctx) tpA :=
   match e in OExpr _ A return OExpr (ctxInsert w tpW ctx) A with
   | Var v => Var (weakenOVar w tpW v)
   | Embed a => Embed a
@@ -188,8 +196,8 @@ Fixpoint weakenOExpr w tpW {ctx A} (e:OExpr ctx A)
   end.
 
 (* Correctness of weakenOExpr: it is equivalent to weaken_pfun *)
-Lemma weakenOExpr_correct w tpW {ctx A} (e:OExpr ctx A) :
-  exprSemantics (weakenOExpr w tpW e) =o=
+Lemma weakenOExpr_correct w {W RW} tpW {ctx A RA tpA} (e:@OExpr ctx A RA tpA) :
+  exprSemantics (@weakenOExpr w W RW tpW ctx A RA tpA e) =o=
   compose_pfun (weaken_pfun w tpW ctx) (exprSemantics e).
   revert w; induction e; intros; simpl.
   - apply weakenOVar_correct.
@@ -202,8 +210,8 @@ Lemma weakenOExpr_correct w tpW {ctx A} (e:OExpr ctx A) :
 Qed.
 
 (* Proper-ness of weakenOExpr *)
-Instance Proper_weakenOExpr w tpW {ctx A} :
-  Proper (oexpr_R ==> oexpr_R) (@weakenOExpr w tpW ctx A).
+Instance Proper_weakenOExpr w W RW tpW ctx A RA tpA :
+  Proper (oexpr_R ==> oexpr_R) (@weakenOExpr w W RW tpW ctx A RA tpA).
 Proof.
   intros e1 e2 Re. unfold oexpr_R.
   etransitivity; [ apply weakenOExpr_correct | ].
@@ -212,8 +220,8 @@ Proof.
 Qed.
 
 (* Proper-ness of weakenOExpr *)
-Instance Proper_weakenOExpr_equiv w tpW {ctx A} :
-  Proper (oexpr_eq ==> oexpr_eq) (@weakenOExpr w tpW ctx A).
+Instance Proper_weakenOExpr_equiv w W RW tpW ctx A RA tpA :
+  Proper (oexpr_eq ==> oexpr_eq) (@weakenOExpr w W RW tpW ctx A RA tpA).
 Proof.
   intros e1 e2 Re. unfold oexpr_eq.
   etransitivity; [ apply weakenOExpr_correct | ].
@@ -227,17 +235,18 @@ Qed.
  ***)
 
 (* Substitution for ordered expression variables *)
-Fixpoint substOVar n {ctx A} :
-  OVar A ctx -> OExpr (ctxSuffix n ctx) (ctxNth n ctx) ->
-  OExpr (ctxDelete n ctx) A :=
+Fixpoint substOVar n {ctx A RA tp} :
+  @OVar A RA tp ctx -> OExpr (ctxSuffix n ctx) (ctxNthExpr n ctx) ->
+  OExpr (ctxDelete n ctx) tp :=
   match n return
-        OVar A ctx -> OExpr (ctxSuffix n ctx) (ctxNth n ctx) ->
-        OExpr (ctxDelete n ctx) A
+        OVar tp ctx -> OExpr (ctxSuffix n ctx) (ctxNthExpr n ctx) ->
+        OExpr (ctxDelete n ctx) tp
   with
   | 0 =>
     fun v =>
       match v in OVar _ ctx return
-            OExpr (ctxSuffix 0 ctx) (ctxNth 0 ctx) -> OExpr (ctxDelete 0 ctx) A
+            OExpr (ctxSuffix 0 ctx) (ctxNthExpr 0 ctx) ->
+            OExpr (ctxDelete 0 ctx) tp
       with
       | OVar_0 => fun s => s
       | OVar_S v' => fun _ => Var v'
@@ -245,18 +254,18 @@ Fixpoint substOVar n {ctx A} :
   | S n' =>
     fun v =>
       match v in OVar _ ctx return
-            OExpr (ctxSuffix (S n') ctx) (ctxNth (S n') ctx) ->
-            OExpr (ctxDelete (S n') ctx) A
+            OExpr (ctxSuffix (S n') ctx) (ctxNthExpr (S n') ctx) ->
+            OExpr (ctxDelete (S n') ctx) tp
       with
       | OVar_0 => fun _ => Var OVar_0
-      | @OVar_S _ ctx' B v' =>
-        fun s => weakenOExpr 0 B (substOVar n' v' s)
+      | @OVar_S _ _ _ B RB tpB ctx' v' =>
+        fun s => weakenOExpr 0 tpB (substOVar n' v' s)
       end
   end.
-Arguments substOVar !n {ctx A} !v s.
+Arguments substOVar !n {ctx A RA tp} !v s.
 
 (* Correctness of substOVar: it is equivalent to subst_pfun *)
-Lemma substOVar_correct n {ctx A} (v:OVar A ctx) s :
+Lemma substOVar_correct n {ctx A RA tp} (v:@OVar A RA tp ctx) s :
   exprSemantics (substOVar n v s) =o=
   compose_pfun (subst_pfun ctx n (exprSemantics s)) (varSemantics v).
 Proof.
@@ -271,8 +280,8 @@ Proof.
 Qed.
 
 (* substOVar is Proper in its s argument *)
-Instance Proper_substOVar n {ctx A} v :
-  Proper (oexpr_R ==> oexpr_R) (@substOVar n ctx A v).
+Instance Proper_substOVar n {ctx A RA tp} v :
+  Proper (oexpr_R ==> oexpr_R) (@substOVar n ctx A RA tp v).
 Proof.
   revert ctx v; induction n; intros; destruct v; intros e1 e2 Re; simpl.
   - assumption.
@@ -282,8 +291,8 @@ Proof.
 Qed.
 
 (* substOVar is Proper in its s argument *)
-Instance Proper_substOVar_equiv n {ctx A} v :
-  Proper (oexpr_eq ==> oexpr_eq) (@substOVar n ctx A v).
+Instance Proper_substOVar_equiv n {ctx A RA tp} v :
+  Proper (oexpr_eq ==> oexpr_eq) (@substOVar n ctx A RA tp v).
 Proof.
   intros e1 e2 Re; destruct Re; split; apply Proper_substOVar; assumption.
 Qed.
@@ -294,18 +303,18 @@ Qed.
  ***)
 
 (* Substitution for ordered expressions *)
-Fixpoint substOExpr n {ctx A} (e:OExpr ctx A) :
-  OExpr (ctxSuffix n ctx) (ctxNth n ctx) -> OExpr (ctxDelete n ctx) A :=
+Fixpoint substOExpr n {ctx A RA tp} (e:@OExpr ctx A RA tp) :
+  OExpr (ctxSuffix n ctx) (ctxNthExpr n ctx) -> OExpr (ctxDelete n ctx) tp :=
   match e with
   | Var v => fun s => substOVar n v s
   | Embed a => fun _ => Embed a
   | App e1 e2 => fun s => App (substOExpr n e1 s) (substOExpr n e2 s)
   | Lam e => fun s => Lam (substOExpr (S n) e s)
   end.
-Arguments substOExpr n {ctx A} !e.
+Arguments substOExpr n {ctx A RA tp} !e.
 
 (* Correctness of substOExpr: it is equivalent to subst_pfun *)
-Lemma substOExpr_correct n {ctx A} (e:OExpr ctx A) s :
+Lemma substOExpr_correct n {ctx A RA tp} (e:@OExpr ctx A RA tp) s :
   exprSemantics (substOExpr n e s) =o=
   compose_pfun (subst_pfun ctx n (exprSemantics s)) (exprSemantics e).
 Proof.
@@ -322,8 +331,13 @@ Proof.
 Qed.
 
 
+(***
+ *** OExpr Rewrite Rules
+ ***)
+
 (* The Beta rule for ordered expressions *)
-Lemma OExpr_Beta ctx A B (e1: OExpr (CtxCons A ctx) B) (e2: OExpr ctx A) :
+Lemma OExpr_Beta ctx A RA tpA B RB tpB
+      (e1: @OExpr (@CtxCons A RA tpA ctx) B RB tpB) (e2: @OExpr ctx A RA tpA) :
   App (Lam e1) e2 =e= substOExpr 0 e1 e2.
 Proof.
   unfold oexpr_eq; simpl.
@@ -331,6 +345,320 @@ Proof.
   rewrite pfun_apply_pfun_curry; try typeclasses eauto.
   f_equiv.
 Qed.
+
+(*
+(* The OExpr for the fst function *)
+Definition OFst {ctx A RA B} {RB:OTRelation B} {tp} : @OExpr ctx (A*B -o> A) _ tp :=
+  Embed (tp:=tp) (@ofst A B RA RB).
+
+(* The OExpr for the snd function *)
+Definition OSnd {ctx A B} : OExpr ctx (OTpArrow (OTpPair A B) B) :=
+  Embed (A:=OTpArrow (OTpPair A B) B) osnd.
+
+(* The OExpr for the pair function *)
+Definition OPair {ctx A B} : OExpr ctx (OTpArrow A (OTpArrow B (OTpPair A B))) :=
+  Embed (A:=OTpArrow A (OTpArrow B (OTpPair A B))) opair.
+
+(* Mark the above OExpr constructs as opaque *)
+Typeclasses Opaque OFst OSnd OPair.
+*)
+
+Lemma OExpr_fst_pair ctx A RA tpA B RB tpB
+      (e1: @OExpr ctx A RA tpA) (e2: @OExpr ctx B RB tpB) :
+  App (Embed ofst) (App (App (Embed opair) e1) e2) =e= e1.
+Proof.
+  split; intros a1 a2 Ra; simpl; f_equiv; assumption.
+Qed.
+
+Lemma OExpr_snd_pair ctx A RA tpA B RB tpB
+      (e1: @OExpr ctx A RA tpA) (e2: @OExpr ctx B RB tpB) :
+  App (Embed osnd) (App (App (Embed opair) e1) e2) =e= e2.
+Proof.
+  split; intros a1 a2 Ra; simpl; f_equiv; assumption.
+Qed.
+
+Lemma OExpr_pair_eta ctx A RA (tpA:@OTypeExpr A RA) B RB (tpB:@OTypeExpr B RB)
+      (e: OExpr ctx (OTpPair tpA tpB)) :
+  (App (App (Embed opair) (App (Embed ofst) e)) (App (Embed osnd) e)) =e= e.
+Proof.
+  split; intros a1 a2 Ra; split; simpl; f_equiv; f_equiv; assumption.
+Qed.
+
+Hint Rewrite OExpr_fst_pair OExpr_snd_pair OExpr_pair_eta : osimpl.
+
+
+(***
+ *** Quoting Tactic for Ordered Expressions
+ ***)
+
+(* Specially-marked versions of fst and snd just used for quoting OExprs *)
+Definition celem_head {ctx A RA tpA}
+           (celem: CtxElem (@CtxCons A RA tpA ctx)) : A :=
+  let (_,head) := celem in head.
+Definition celem_rest {ctx A RA tpA}
+           (celem: CtxElem (@CtxCons A RA tpA ctx)) : CtxElem ctx :=
+  let (rest,_) := celem in rest.
+
+(* Typeclass for incrementally quoting functions into OExpr variables, by
+peeling off the celem_rest projections one at a time and adding them as OVar_S
+constructors to the input variable to build the output variable *)
+Class QuotesToVar {ctx1 ctx2 A RA} {tpA:@OTypeExprInd A RA}
+      (f: CtxElem ctx1 -> CtxElem ctx2)
+      (vin: OVar tpA ctx2) (vout: OVar tpA ctx1) : Prop :=
+  quotesToVar :
+    forall c, varSemantics vin @o@ (f c) = varSemantics vout @o@ c.
+
+Instance QuotesToVar_Base {ctx A RA} {tpA:@OTypeExprInd A RA}
+         (v:@OVar A RA tpA ctx) : QuotesToVar (fun c => c) v v.
+Proof.
+  intro; reflexivity.
+Qed.
+
+Instance QuotesToVar_Step {ctx1 ctx2 A RA} {tpA:@OTypeExprInd A RA}
+         {B RB} {tpB:@OTypeExprInd B RB}
+         (f: CtxElem ctx1 -> CtxElem (@CtxCons B RB tpB ctx2)) vin vout
+         (q: @QuotesToVar _ _ A RA tpA f (OVar_S vin) vout) :
+  QuotesToVar (fun c => celem_rest (f c)) vin vout.
+Proof.
+  intro. apply q.
+Qed.
+
+
+(* Class for quoting functions to OExprs *)
+Class QuotesTo {ctx A RA} {tpA:@OTypeExprInd A RA} (f: CtxElem ctx -> A)
+      (e: @OExpr ctx A RA tpA) : Prop :=
+  quotesTo : forall c, f c =o= exprSemantics e @o@ c.
+
+(* Logically the same as QuotesTo, but we never build lambdas in this one, i.e.,
+this only builds "atomic" OExprs *)
+Class QuotesToAtomic {ctx A RA} {tpA:@OTypeExprInd A RA}
+      (f: CtxElem ctx -> A) (e: @OExpr ctx A RA tpA) :=
+  quotesToAtomic : QuotesTo f e.
+
+(* Quote any term of functional type to a lambda *)
+Instance QuotesTo_Lam {ctx A RA} {tpA:@OTypeExprInd A RA}
+         {B RB} {tpB:@OTypeExprInd B RB} (f: CtxElem ctx -> A -o> B)
+         (e: OExpr (CtxCons tpA ctx) tpB)
+         (q: QuotesTo (fun c => f (celem_rest c) @o@ (celem_head c)) e) :
+  QuotesTo f (Lam e) | 2.
+Proof.
+  intros; split; intro; intros; simpl; rewrite H;
+    rewrite <- (q (c,a2)); reflexivity.
+Qed.
+
+(* Special case: quote ofuns as lambdas, destructuring the ofun *)
+Instance QuotesTo_Lam_ofun {ctx A RA} {tpA:@OTypeExprInd A RA}
+         {B RB} {tpB:@OTypeExprInd B RB} (f: CtxElem ctx -> A -> B) prp
+         (e: OExpr (CtxCons tpA ctx) tpB)
+         (q: QuotesTo (fun c => f (celem_rest c) (celem_head c)) e) :
+  QuotesTo (fun c => ofun (f c) (prp:=prp c)) (Lam e) | 1.
+Proof.
+  apply QuotesTo_Lam. assumption.
+Qed.
+
+
+(* Quote any non-function term as an atomic OExpr *)
+Instance QuotesTo_Atomic {ctx A RA} {tpA:@OTypeExprInd A RA}
+         (f: CtxElem ctx -> A) e (q: QuotesToAtomic f e) :
+  QuotesTo (tpA:=tpA) f e | 3 := q.
+
+(* Quote any use of celem_head as a var *)
+Instance QuotesTo_Var {ctx1 ctx2 A RA} {tpA:@OTypeExprInd A RA}
+         (f: CtxElem ctx1 -> CtxElem (CtxCons tpA ctx2)) v
+         (q: QuotesToVar f OVar_0 v) :
+  QuotesToAtomic (fun c => celem_head (f c)) (Var v) | 1.
+Proof.
+  intro. rewrite <- (quotesToVar (QuotesToVar:=q)). destruct (f c).
+  reflexivity.
+Qed.
+
+(* Special case for an eta-reduced celem_head application *)
+Instance QuotesTo_Var0 {ctx A RA} {tpA:@OTypeExprInd A RA} :
+  QuotesToAtomic (@celem_head ctx A RA tpA) (Var OVar_0) | 1.
+Proof.
+  intro; reflexivity.
+Qed.
+
+(* Quote applications as OExpr applications, where the function must still be
+atomic but the argument need not be *)
+Instance QuotesTo_App {ctx A RA} {tpA:@OTypeExprInd A RA} {B RB}
+         {tpB:@OTypeExprInd B RB}
+         (f1: CtxElem ctx -> A -o> B) (f2: CtxElem ctx -> A)
+         (e1: OExpr ctx (OTpArrow tpA tpB)) (e2: OExpr ctx tpA)
+         (q1: QuotesToAtomic f1 e1) (q2: QuotesTo f2 e2) :
+  QuotesToAtomic (fun c => (f1 c) @o@ (f2 c)) (App e1 e2) | 1.
+Proof.
+  intro. simpl. f_equiv.
+  - apply (quotesTo (QuotesTo:=q1)).
+  - apply (quotesTo (QuotesTo:=q2)).
+Qed.
+
+(* Quote ofuns in atomic position as lambdas *)
+Instance QuotesToAtomic_ofun {ctx A RA} {tpA:@OTypeExprInd A RA} {B RB}
+         {tpB:@OTypeExprInd B RB} (f: CtxElem ctx -> A -> B) prp
+         (e: OExpr (CtxCons tpA ctx) tpB)
+         (q: QuotesTo (fun c => f (celem_rest c) (celem_head c)) e) :
+  QuotesToAtomic (fun c => ofun (f c) (prp:=prp c)) (Lam e) | 1.
+Proof.
+  apply QuotesTo_Lam. assumption.
+Qed.
+
+(* Quote objects that are independent of the context as embedded objects, but at
+low priority *)
+Instance QuotesTo_Embed {ctx A RA} {tpA:@OTypeExprInd A RA} (a:A) :
+  QuotesToAtomic (fun _ => a) (@Embed ctx A RA tpA a) | 2.
+Proof.
+  intro. reflexivity.
+Qed.
+
+(* Quote pairs as applications of opair *)
+Instance QuotesTo_pair {ctx A RA} {tpA:@OTypeExprInd A RA} {B RB}
+         {tpB:@OTypeExprInd B RB} (a: CtxElem ctx -> A) (b: CtxElem ctx -> B)
+         (e1: OExpr ctx tpA) (e2: OExpr ctx tpB)
+         (q1: QuotesTo a e1) (q2: QuotesTo b e2) :
+  QuotesToAtomic (tpA:=OTpPair tpA tpB) (fun c => (a c, b c))
+                 (App (App (Embed opair) e1) e2) | 1.
+Proof.
+  intro. simpl. rewrite (q1 c). rewrite (q2 c). reflexivity.
+Qed.
+
+(* Quote applications of fst as applications of ofst *)
+Instance QuotesTo_fst {ctx A RA} {tpA:@OTypeExprInd A RA} {B RB}
+         {tpB:@OTypeExprInd B RB} (f: CtxElem ctx -> A * B)
+         (e: OExpr ctx (OTpPair tpA tpB)) (q: QuotesTo f e) :
+  QuotesToAtomic (tpA:=tpA) (fun c => fst (f c)) (App (Embed ofst) e) | 1.
+Proof.
+  intro. simpl. rewrite (q c). reflexivity.
+Qed.
+
+(* Quote applications of snd as applications of osnd *)
+Instance QuotesTo_snd {ctx A RA} {tpA:@OTypeExprInd A RA} {B RB}
+         {tpB:@OTypeExprInd B RB} (f: CtxElem ctx -> A * B)
+         (e: OExpr ctx (OTpPair tpA tpB)) (q: QuotesTo f e) :
+  QuotesToAtomic (tpA:=tpB) (fun c => snd (f c)) (App (Embed osnd) e) | 1.
+Proof.
+  intro. simpl. rewrite (q c). reflexivity.
+Qed.
+
+
+(* Use QuotesTo to prove a relation *)
+Lemma oquote_R {A RA} {tpA:@OTypeExprInd A RA} {f1 f2 : A}
+      {e1 e2: OExpr CtxNil tpA}
+      {q1: QuotesTo (fun _ => f1) e1} {q2: QuotesTo (fun _ => f2) e2} :
+  e1 <e= e2 -> f1 <o= f2.
+Proof.
+  intro R12.
+  etransitivity; [ apply (q1 tt) | ].
+  etransitivity; [ | apply (q2 tt) ].
+  apply R12. reflexivity.
+Qed.
+
+(* Use QuotesTo to prove an equivalence *)
+Lemma oquote_eq {A RA} {tpA:@OTypeExpr A RA} {f1 f2 : A}
+      {e1 e2: OExpr CtxNil tpA}
+      {q1: QuotesTo (tpA:=tpA) (fun _ => f1) e1} {q2: QuotesTo (fun _ => f2) e2} :
+  e1 =e= e2 -> f1 =o= f2.
+Proof.
+  intro R12.
+  etransitivity; [ apply (q1 tt) | ].
+  etransitivity; [ | symmetry; apply (q2 tt) ].
+  f_equiv. apply R12.
+Qed.
+
+
+(* Translate a problem about proper functions into one about OExprs, by
+"quoting" both sides *)
+Ltac oquote :=
+  lazymatch goal with
+  | |- ?e1 =o= ?e2 =>
+    apply oquote_eq
+  | |- ?e1 <o= ?e2 =>
+    apply oquote_R
+  end.
+
+Ltac oexpr_simpl :=
+  rewrite_strat (bottomup (choice (OExpr_Beta ; eval simpl) (hints osimpl))).
+
+(* Translate a problem about proper functions into one about OExprs by calling
+oquote, simplify both sides using the osimpl rewrite database, and then try to
+use reflexivity, going back to proper functions if that does not work *)
+Ltac osimpl :=
+  simpl; oquote; try oexpr_simpl; try reflexivity; try typeclasses eauto; simpl.
+
+
+(***
+ *** Testing the Quote Mechanism
+ ***)
+
+Module OQuoteTest.
+
+(* Set Printing All. *)
+(* Hint Extern 4 (QuotesTo ) : typeclass_instances. *)
+
+(*
+Goal (forall A (RA:OTRelation A) (a:A),
+         exists (tpA:OTypeExprInd A) (e:OExpr CtxNil tpA),
+           QuotesTo (fun _ => a) e).
+  intros. eexists. eexists.
+  typeclasses eauto.
+  simple apply @QuotesTo_Atomic.
+ *)
+(* Hint Extern 1 (OTypeExprInd _) => prove_OTypeExpr : typeclass_instances. *)
+(* Typeclasses Opaque OTypeExprInd.
+Print HintDb typeclass_instances. *)
+
+Instance Equivalence_oexpr_eq' ctx A RA (tp:@OTypeExprInd A RA)
+  : Equivalence (@oexpr_eq ctx A RA tp) := Equivalence_oexpr_eq _ _ _ _.
+
+(* A simple test case for constant terms *)
+Lemma simple_quote_test A `{OType A} a : a =o= a.
+  osimpl.
+Qed.
+
+(* A simple test case with all 4 OExpr constructs, that does beta-reduction *)
+Lemma beta_test A `{OType A} a : (ofun (A:=A) (fun x => x)) @o@ a =o= a.
+  osimpl.
+Qed.
+
+(* A test case with the first projection of a product *)
+Lemma product_proj1_test A `{OType A} B `{OType B} (a:A) (b:B) :
+  ofst @o@ (a ,o, b) =o= a.
+  osimpl.
+Qed.
+
+(* A test case with with beta-reduction and projections + eta for products *)
+Lemma beta_product_test A `{OType A} B `{OType B} (p:A*B) :
+  ofun (fun p => (osnd @o@ p ,o, ofst @o@ p)) @o@ (osnd @o@ p ,o, ofst @o@ p)
+  =o= p.
+  (* osimpl *)
+  (* NOTE: we write this out to see how long each step takes... *)
+  oquote.
+
+  FIXME HERE NOW: quoting for ofuns is not working!
+
+  oexpr_simpl. reflexivity. typeclasses eauto.
+Qed.
+
+Lemma double_lambda_test A `{OType A} :
+  (ofun (fun (f : A -o> A) => ofun (fun x => f @o@ x))) @o@ (ofun (fun y => y))
+  =o= ofun (fun x => x).
+  osimpl.
+Qed.
+
+(* A test case with with beta-reduction and projections for products *)
+Lemma beta_product_test2 A `{OType A} B `{OType B} :
+  ofun (fun a =>
+          ofun (fun b =>
+                  ofun (fun p => (osnd @o@ p ,o, ofst @o@ p)) @o@ (b ,o, a)))
+  =o= opair.
+  (* osimpl *)
+  (* NOTE: we write this out to see how long each step takes... *)
+  oquote. oexpr_simpl.
+  reflexivity. typeclasses eauto. typeclasses eauto.
+Qed.
+
+End OQuoteTest.
+
 
 
 FIXME HERE NOW: continue porting OExpr_typed.v!
